$F(n)=F(n-3)*n, n>2$
$F(2) = 1$
$F(1) = 1$
$F(0) = 1$
$M(n)=M(n-3)+1, n>2$
$M(2)=0$
$M(1)=0$
$M(0)=0$
$M(n)=M(n-3)+1$
$M(n)=(M(n-4)+1)+1=M(n-4)+2$
$M(n)=(M(n-5)+1)+2=M(n-5)+3$
$M(n)=M(n-i)+\lceil \frac{i}{3} \rceil$
$n-i=0$
$n=i$


$F(n)=F\left( \frac{n}{2} \right) + 1, n>1$
$F(0)=1$
$F(1)=1$
$M(n)=M\left( \frac{n}{2} \right) +1,n>1$
$M(0)=1$
$M(1)=1$\
$M(n)=M\left( \frac{n}{2} \right)+1$
$M(n)=(M\left( \frac{n-1}{2} \right)+1)+1=M\left( \frac{n-1}{2} \right)+2$
$M(n)=(M\left( \frac{n-2}{2} \right)+1)+2=M\left( \frac{n-2}{2} \right)+3$
$M(n)=M\left( \frac{n-i}{2} \right)+1+i$
$\frac{n-i}{2}=1$
$n-i=2$
$n-2=i$
$M(n)=M(1)+1+n-2$
$M(n)=1+1+n-2$
$M(n)=n$

$F(n)=F(n-2)*n, n>1$
$F(1)=1$
$F(0)=1$
$M(n)=M(n-2)+1, n>1$
$M(1)=1$
$M(0)=1$
$M(n)=M(n-2)+1$
$M(n)=M(n-3)+2$
$M(n)=M(n-4)+3$
$M(n)=M(n-i)+i-1$
$n-i=0$
$n=i$
$M(n)=M(0)+n-1$
$M(n)=n$

$F(n)=F(n-2)*n, n>1$
$F(0)=1,C(0)=0$
$F(1)=1, C(1)=0$
$F(2)=F(0)*2, C(2)=C(0)+1=0+1=1$
$F(3)=F(1)*2, C(3)=C(1)+1=0+1=1$
$F(4)=F(2)*4,C(4)=C(2)+1=1+1=2$
$F(5)=F(3)*5,C(5)=C(3)+1=1+1=2$


$F(n)=F\left( \frac{n}{2} \right)+1,n>1$
$F(0)=1, C(0)=0$
$F(1)=1,C(1)=0$
$F(2)=F(1)+1,C(2)=C(1)+1=0+1=1$
$F(3)=F(1)+1,C(3)=C(1)+1=0+1=1$

$F(n)=F(n-3)*n,n>2$
$F(0)=1,C(0)=0$
$F(1)=1,C(1)=0$
$F(2)=1,C(2)=0$
$F(3)=F(0)*3,C(3)=C(0)+1=0+1=1$
$F(4)=F(1)*3,C(4)=C(1)+1=0+1=1$
$F(5)=F(2)*3,C(5)=C(2)+1=0+1=1$
$F(6)=F(3)*3,C(6)=C(3)+1=1+1=2$
